platform/cito/GoodModule.v
@@ -5,33 +5,5 @@ Record GoodModule :=
   {
     Name : string;
     Functions : list GoodFunction;
-    NoDupFuncNames : NoDup (map (fun f => SyntaxFunc.Name (proj1_sig f)) Functions)
+    NoDupFuncNames : NoDup (map GoodFunction.Name Functions)
   }.
-
-Require Import SyntaxModule.
-Definition is_good_module module := 
-  NoDup (map SyntaxFunc.Name (SyntaxModule.Functions module)) /\
-  List.Forall GoodFunc (Functions module).
-
-Definition to_prod_list : forall A P (ls : list A), List.Forall P ls -> list { x | P x }.
-  induction ls.
-  econstructor 1.
-  econstructor 2.
-  econstructor; inversion H; subst; eauto.
-  eapply IHls; inversion H; subst; eauto.
-Defined.
-
-Lemma to_prod_list_proj1 : forall A ls P (H : List.Forall P ls), List.map (@proj1_sig _ P)(@to_prod_list A _ _ H) = ls.
-  induction ls; simpl; intuition.
-Qed.
-
-Definition to_good_module m : is_good_module m -> GoodModule.
-  intros.
-  destruct H.
-  econstructor.
-  eapply (SyntaxModule.Name m).
-  instantiate (1 := to_prod_list H0).
-  erewrite <- map_map.
-  erewrite to_prod_list_proj1.
-  eauto.
-Defined.
